exec api

VCVio/OracleComp/OracleAlg.lean
@@ -17,24 +17,60 @@ The function `OracleAlg.exec` can then be used to properly "execute" a compuatio
 according to the specified simulation oracle
 -/
 
+open OracleSpec OracleComp
+
 structure OracleAlg (spec : OracleSpec) where
   baseState : Type
-  initState : baseState
+  init_state : baseState
   baseSimOracle : spec →[baseState]ₛₒ unifSpec
 
 namespace OracleAlg
 
 variable {spec : OracleSpec} {α β γ : Type}
 
--- @[inline, reducible]
 def exec (alg : OracleAlg spec) (oa : OracleComp spec α) : OracleComp unifSpec α :=
-  simulate' alg.baseSimOracle oa alg.initState
+  simulate' alg.baseSimOracle oa alg.init_state
 
-end OracleAlg
+lemma exec.def (alg : OracleAlg spec) (α : Type) :
+    alg.exec (α := α) = (simulate' alg.baseSimOracle · alg.init_state) := rfl
+
+@[simp]
+lemma exec_pure (alg : OracleAlg spec) (x : α) : alg.exec (pure x) = pure x := rfl
+
+@[simp]
+lemma exec_bind (alg : OracleAlg spec) (oa : OracleComp spec α) (ob : α → OracleComp spec β) :
+    alg.exec (oa >>= ob) = (do
+      let z ← simulate alg.baseSimOracle oa alg.init_state
+      simulate' alg.baseSimOracle (ob z.1) z.2) :=
+  simulate'_bind alg.baseSimOracle oa ob alg.init_state
+
+@[simp]
+lemma exec_query (alg : OracleAlg spec) (i : spec.ι) (t : spec.domain i) :
+    alg.exec (query i t) = Prod.fst <$> alg.baseSimOracle i (t, alg.init_state) :=
+  simulate'_query alg.baseSimOracle i t alg.init_state
+
+@[simp]
+lemma exec_map (alg : OracleAlg spec) (oa : OracleComp spec α) (f : α → β) :
+    alg.exec (f <$> oa) = f <$> alg.exec oa :=
+  simulate'_map alg.baseSimOracle oa f alg.init_state
+
+-- @[simp]
+-- lemma exec_seq (alg : OracleAlg spec) (oa : OracleComp spec α)
+
+section baseOracleAlg
 
 /-- Simple base structure for defining algorithms using only uniform selection oracles.
 Usefull to auto-fill in fields with simple defaults in this case. -/
+@[inline, reducible]
 def baseOracleAlg : OracleAlg unifSpec where
   baseState := Unit
-  initState := ()
+  init_state := ()
   baseSimOracle := idOracle
+
+@[simp]
+lemma exec_baseOracleAlg : baseOracleAlg.exec (α := α) = id := by
+  simp only [exec.def, idOracle.simulate'_eq, Function.funext_iff, id_eq, implies_true]
+
+end baseOracleAlg
+
+end OracleAlg
